Coq/src/CertGraph.v
@@ -1,0 +1,585 @@
+Require Import Omega.
+Require Import Program.Basics.
+From hahn Require Import Hahn.
+From promising Require Import Basic.
+From imm Require Import Events Execution
+     Traversal TraversalConfig SimTraversal SimTraversalProperties
+     Prog ProgToExecution ProgToExecutionProperties Receptiveness
+     imm_common imm_s imm_s_hb SimulationRel
+     CertExecution2 CertExecutionMain
+     SubExecution CombRelations AuxRel.
+Require Import AuxRel AuxDef EventStructure LblStep CertRf.
+Require Import Coq.Logic.FunctionalExtensionality Classical_Prop.
+
+Set Implicit Arguments.
+Local Open Scope program_scope.
+
+Section CertGraph.
+  Variable prog : Prog.t.
+  Variable G  : execution.
+  Variable GPROG : program_execution prog G.
+  Variable sc : relation actid.
+  Variable TC : trav_config.
+  Variable TC': trav_config.
+  Variable thread : thread_id.
+  Variable state : state.
+    
+  Notation "'certG'" := state.(ProgToExecution.G).
+
+  Notation "'certE'" := certG.(acts_set).
+
+  Definition certLab (e : actid) : label :=
+    if excluded_middle_informative (certE e)
+    then certG.(lab) e
+    else G.(lab) e.
+
+  Notation "'certRmw'" := (certG.(rmw)).
+
+  Notation "'new_rf'" := (cert_rf G sc TC' thread).
+
+  Notation "'E'" := G.(acts_set).
+
+  Notation "'R'" := (fun a => is_true (is_r G.(lab) a)).
+  Notation "'W'" := (fun a => is_true (is_w G.(lab) a)).
+  Notation "'F'" := (fun a => is_true (is_f G.(lab) a)).
+
+  Notation "'Rel'" := (fun a => is_true (is_rel G.(lab) a)).
+
+  Notation "'R_ex'" := (fun a => R_ex G.(lab) a).
+  
+  Notation "'sb'" := (G.(sb)).
+  Notation "'rmw'" := G.(rmw).
+  Notation "'addr'" := G.(addr).
+  Notation "'data'" := G.(data).
+  Notation "'ctrl'" := G.(ctrl).
+  Notation "'rmw_dep'" := G.(rmw_dep).
+  Notation "'rf'" := (G.(rf)).
+  Notation "'co'" := (G.(co)).
+  
+  Notation "'ppo'" := (G.(ppo)).
+  Notation "'hb'" := (G.(imm_s_hb.hb)).
+  Notation "'vf'" := (furr G sc).
+
+  Notation "'C'"  := (covered TC).
+  Notation "'I'"  := (issued TC).
+  Notation "'C''"  := (covered TC').
+  Notation "'I''"  := (issued TC').
+
+  (* Notation "'E0'" := (E0 G TC' thread).  *)
+  (* Notation "'D'" := (D G TC' thread). *)
+  
+  Notation "'E0'" := (Tid_ thread ∩₁ (C' ∪₁ dom_rel (sb^? ⨾ ⦗ I' ⦘))).
+  Notation "'D'" := (D G TC' thread).
+
+  Record cert_graph :=
+    { cslab : eq_dom ((Tid_ thread) ∩₁ (C' ∪₁ I')) certLab G.(lab);
+      cuplab_cert : forall e (EE : certE e),
+          same_label_up_to_value (certG.(lab) e) (G.(lab) e);
+      
+      dcertE : certE ≡₁ E0;
+      dcertRMW : certRmw ≡ ⦗ certE ⦘ ⨾ rmw ⨾ ⦗ certE ⦘;
+      
+      new_rfv : new_rf ⊆ same_val certLab;
+      new_rfl : new_rf ⊆ same_loc certLab;
+      new_rf_iss_sb : new_rf ⊆ ⦗ I ⦘ ⨾ new_rf ∪ sb;
+
+      oval : eq_dom D (val certLab) (val G.(lab));
+    }.
+
+  Section CertGraphProperties.
+    Variable WF : Wf G.
+    Variable Wf_sc : wf_sc G sc.
+    Variable IMMC : imm_consistent G sc.
+    Variable TCCOH : tc_coherent G sc TC.
+    Variable TSTEP : isim_trav_step G sc thread TC TC'.
+
+    Fact TCCOH' : tc_coherent G sc TC'.
+    Proof. 
+      eapply sim_trav_step_coherence; red; eauto.
+    Qed.
+
+    Hint Resolve TCCOH'. 
+
+    Lemma trstep_thread_prog : IdentMap.In thread prog. 
+    Proof. 
+      apply sim_trav_step_to_step in TSTEP. 
+      destruct TSTEP as [e [T'' ITSTEP]]. desf. 
+      assert (E e) as EE.
+      { cdes ITSTEP. desf.
+        { apply COV. }
+        apply ISS. }
+      set (BB := EE).
+      apply GPROG in BB.
+      desf. exfalso.
+      cdes ITSTEP. desf.
+      { apply NEXT. by eapply init_covered; eauto. }
+      apply NISS. by eapply init_issued; eauto. 
+    Qed.
+
+    (* Lemma E0_eq_certE  *)
+    (*       (TEH : thread_restricted_execution G thread certG)  *)
+    (*       (CDOM : certE ⊆₁ C) :  *)
+    (*   E0 ≡₁ certE. *)
+    (* Proof.  *)
+    (*   red. split.  *)
+    (*   { (* E0_in_e in CertRF ? *) *)
+    (*     rewrite tr_acts_set; eauto. *)
+    (*     rewrite set_interC. *)
+    (*     apply set_subset_inter; auto. *)
+    (*     rewrite coveredE; eauto. *)
+    (*     rewrite issuedE; eauto. *)
+    (*     rewrite wf_sbE. *)
+    (*     basic_solver. } *)
+    (*   apply set_subset_inter_r. split. *)
+    (*   { etransitivity.  *)
+    (*     { eapply TEH.(tr_acts_set). }         *)
+    (*     basic_solver. } *)
+    (*   unionR left. *)
+    (*   etransitivity; eauto.   *)
+    (*   eapply sim_trav_step_covered_le. red. eauto.  *)
+    (* Qed. *)
+
+    Lemma E0_eq_certE 
+          (TEH : thread_restricted_execution G thread certG) :
+      E0 ⊆₁ certE.
+    Proof. 
+      rewrite tr_acts_set; eauto.
+      rewrite set_interC.
+      apply set_subset_inter; auto.
+      rewrite coveredE; eauto.
+      rewrite issuedE; eauto.
+      rewrite wf_sbE.
+      basic_solver.
+    Qed.
+
+    (* Lemma E0_in_E : E0 ⊆₁ E. *)
+    (* Proof.  *)
+    (*   rewrite TCCOH'.(coveredE). *)
+    (*   rewrite TCCOH'.(issuedE). *)
+    (*   rewrite wf_sbE. basic_solver.  *)
+    (* Qed. *)
+
+    Lemma E0_eindex_weak e (CTE : E0 e) (NINITT : thread <> tid_init) : 
+      exists index : nat,
+        ⟪ EREP : e = ThreadEvent thread index ⟫.
+    Proof. 
+      ins. destruct CTE as [AA BB].
+      destruct e; simpls; rewrite <- AA in *; desf.
+      eauto. 
+    Qed.
+
+    Lemma E0_eindex 
+          (NINITT : thread <> tid_init)
+          (GPC : wf_thread_state thread state)
+          (TEH : thread_restricted_execution G thread certG) : 
+      exists ctindex,
+        ⟪ CCLOS :forall index (LT : index < ctindex),
+            E0 (ThreadEvent thread index) ⟫ /\
+        ⟪ CREP : forall e (CTE : E0 e),
+            exists index : nat,
+              ⟪ EREP : e = ThreadEvent thread index ⟫ /\
+              ⟪ ILT : index < ctindex ⟫ ⟫.
+    Proof. 
+      assert (E0 ⊆₁ E) as E0_in_E.
+      { eapply E0_in_E; eauto. }
+      destruct (classic (exists e, E0 e)) as [|NCT].
+      2: { exists 0. splits.
+           { ins. inv LT. }
+           ins. exfalso. apply NCT. eauto. }
+      desc.
+      assert (acyclic (sb ⨾ ⦗ E0 ⦘)) as AC.
+      { arewrite (sb ⨾ ⦗E0⦘ ⊆ sb). apply sb_acyclic. }
+      set (doml := filterP E0 G.(acts)).
+      assert (forall c, (sb ⨾ ⦗E0⦘)＊ e c -> In c doml) as UU.
+      { intros c SCC. apply rtE in SCC. destruct SCC as [SCC|SCC].
+        { red in SCC. desf. apply in_filterP_iff. 
+          split; auto. eapply E0_in_E. eauto. }
+        apply inclusion_ct_seq_eqv_r in SCC. apply seq_eqv_r in SCC.
+        apply in_filterP_iff. split; auto; [apply E0_in_E|]; desf. }
+      edestruct (last_exists doml AC UU) as [max [MM1 MM2]].
+      assert (E0 max) as CTMAX.
+      { apply rtE in MM1. destruct MM1 as [MM1|MM1].
+        { red in MM1. desf. }
+        apply inclusion_ct_seq_eqv_r in MM1. apply seq_eqv_r in MM1. desf. }
+      assert (Tid_ thread max) as CTTID by apply CTMAX.
+      destruct max as [l|mthread mindex].
+      { simpls. rewrite <- CTTID in *. desf. }
+      simpls. rewrite CTTID in *.
+      assert (acts_set G (ThreadEvent thread mindex)) as EEM.
+      { by apply E0_in_E. }
+      exists (1 + mindex). splits.
+      { ins. destruct CTMAX as [_ CTMAX].
+        split; [by ins|].
+        apply le_lt_or_eq in LT. destruct LT as [LT|LT].
+        2: { inv LT. }
+        assert (certE (ThreadEvent thread mindex)) as PP.
+        { apply TEH.(tr_acts_set). by split. }
+        assert (E (ThreadEvent thread index)) as EEE.
+        { apply TEH.(tr_acts_set). eapply acts_rep in PP; eauto. desc.
+          eapply GPC.(acts_clos). inv REP. omega. }
+        assert (sb (ThreadEvent thread index) (ThreadEvent thread mindex)) as QQQ.
+        { red.
+          apply seq_eqv_l. split; auto.
+          apply seq_eqv_r. split; auto.
+          red. split; auto. omega. }
+        destruct CTMAX as [AA|[z AA]]; [left|right].
+        { apply TCCOH' in AA. apply AA. eexists.
+          apply seq_eqv_r. split; eauto. }
+        exists z. apply seq_eqv_r in AA. destruct AA as [AA1 AA2].
+        apply seq_eqv_r. split; auto.
+        apply rewrite_trans_seq_cr_cr.
+        { apply sb_trans. }
+        eexists; split; [|by eauto].
+          by apply r_step. }
+      ins. set (CTE' := CTE).
+      apply E0_eindex_weak in CTE'; auto; desc.
+      eexists. splits; eauto.
+      destruct (le_gt_dec index mindex) as [LL|LL].
+      { by apply le_lt_n_Sm. }
+      exfalso.
+      eapply MM2. apply seq_eqv_r. split; [|by apply CTE].
+      red.
+      apply seq_eqv_l. split; auto.
+      apply seq_eqv_r. split; auto.
+      red. rewrite EREP. 
+      split; auto.  
+    Qed.
+
+    Lemma cuplab e (SCG : cert_graph) :
+      same_label_up_to_value (certLab e) (G.(lab) e).
+    Proof.
+      unfold certLab. desf.
+      { by apply SCG. }
+      red. desf.
+    Qed.
+
+    Lemma new_rf_w (SCG : cert_graph) : 
+      new_rf ≡ ⦗ W ⦘ ⨾ new_rf.
+    Proof. rewrite cert_rfD. basic_solver. Qed.
+
+    Lemma new_rf_ntid_iss_sb 
+          (SCG : cert_graph)
+          (IRELCOV : W ∩₁ Rel ∩₁ I ⊆₁ C) :
+      new_rf ⊆ ⦗ NTid_ thread ∩₁ I ⦘ ⨾ new_rf ∪ sb.
+    Proof.
+      etransitivity.
+      { apply cert_rf_ntid_sb; auto. 
+        eapply sim_trav_step_rel_covered; eauto. 
+        eexists; eauto. }
+      sin_rewrite new_rf_iss_sb; auto. 
+      basic_solver 10.
+    Qed.
+
+    Lemma dom_addrE_in_D : dom_rel (addr ⨾ ⦗ E0 ⦘) ⊆₁ D.
+    Proof.
+      rewrite set_inter_union_r.
+      rewrite id_union; relsf; unionL; splits.
+      { rewrite (addr_in_sb WF).
+        generalize (dom_sb_covered TCCOH').
+        unfold CertExecution2.D; basic_solver 21. }
+      arewrite (Tid_ thread ∩₁ dom_rel (sb^? ⨾ ⦗I'⦘) ⊆₁
+                      dom_rel (sb^? ⨾ ⦗I'⦘)) by basic_solver.
+      rewrite dom_rel_eqv_dom_rel.
+      arewrite (⦗I'⦘ ⊆ ⦗W⦘ ⨾ ⦗I'⦘).
+      { generalize (issuedW TCCOH'); basic_solver. }
+      rewrite (dom_l (wf_addrD WF)), !seqA.
+      arewrite (⦗R⦘ ⨾ addr ⨾ sb^? ⨾ ⦗W⦘ ⊆ ppo).
+      { unfold imm_common.ppo; rewrite <- ct_step; basic_solver 12. }
+      unfold CertExecution2.D; basic_solver 21.
+    Qed.
+
+    Lemma dom_ctrlE_in_D : dom_rel (ctrl ⨾ ⦗ E0 ⦘) ⊆₁ D.
+    Proof.
+      rewrite set_inter_union_r.
+      rewrite id_union; relsf; unionL; splits.
+      { rewrite (ctrl_in_sb WF).
+        generalize (dom_sb_covered TCCOH').
+        unfold CertExecution2.D; basic_solver 21. }
+      arewrite (Tid_ thread ∩₁ dom_rel (sb^? ⨾ ⦗I'⦘) ⊆₁
+                      dom_rel (sb^? ⨾ ⦗I'⦘)) by basic_solver.
+      rewrite dom_rel_eqv_dom_rel.
+      arewrite (ctrl ⨾ sb^? ⊆ ctrl).
+      { generalize (ctrl_sb WF); basic_solver 21. }
+      arewrite (⦗I'⦘ ⊆ ⦗W⦘ ⨾ ⦗I'⦘).
+      { generalize (issuedW TCCOH'); basic_solver. }
+      rewrite (wf_ctrlD WF), !seqA.
+      arewrite (⦗R⦘ ⨾ ctrl ⨾ ⦗W⦘ ⊆ ppo).
+      { unfold imm_common.ppo; rewrite <- ct_step; basic_solver 12. }
+      unfold CertExecution2.D; basic_solver 21.
+    Qed.
+
+    Lemma dom_rmw_depE_in_D : dom_rel (rmw_dep ⨾ ⦗ E0 ⦘) ⊆₁ D.
+    Proof.
+      rewrite set_inter_union_r.
+      rewrite id_union; relsf; unionL; splits.
+      { rewrite (rmw_dep_in_sb WF).
+        generalize (dom_sb_covered TCCOH').
+        unfold CertExecution2.D; basic_solver 21. }
+      arewrite (Tid_ thread ∩₁ dom_rel (sb^? ⨾ ⦗I'⦘) ⊆₁
+                      dom_rel (sb^? ⨾ ⦗I'⦘)) by basic_solver.
+      rewrite dom_rel_eqv_dom_rel.
+      rewrite (wf_rmw_depD WF), !seqA.
+      arewrite (⦗I'⦘ ⊆ ⦗W⦘ ⨾ ⦗I'⦘).
+      { generalize (issuedW TCCOH'); basic_solver. }
+      arewrite (⦗R⦘ ⨾ rmw_dep ⨾ ⦗R_ex⦘ ⨾ sb^? ⨾ ⦗W⦘ ⊆ ppo).
+      2: unfold CertExecution2.D; basic_solver 21.
+      unfold imm_common.ppo; hahn_frame.
+      case_refl _.
+      { by rewrite <- ct_step; basic_solver 12. }
+      rewrite ct_begin; rewrite <- inclusion_t_rt, <- ct_step; basic_solver 12.
+    Qed.
+
+    Lemma dom_rmwE_in_D : dom_rel (rmw ⨾ ⦗ E0 ⦘) ⊆₁ D.
+    Proof.
+      rewrite set_inter_union_r.
+      rewrite id_union; relsf; unionL; splits.
+      { rewrite (rmw_in_sb WF).
+        generalize (dom_sb_covered TCCOH').
+        unfold CertExecution2.D; basic_solver 21. }
+      arewrite (Tid_ thread ∩₁ dom_rel (sb^? ⨾ ⦗I'⦘) ⊆₁
+                      dom_rel (sb^? ⨾ ⦗I'⦘)) by basic_solver.
+      rewrite dom_rel_eqv_dom_rel.
+      arewrite (⦗I'⦘ ⊆ ⦗W⦘ ⨾ ⦗I'⦘).
+      { generalize (issuedW TCCOH'); basic_solver. }
+      generalize (rmw_in_ppo WF) (rmw_sb_W_in_ppo WF).
+      unfold CertExecution2.D; basic_solver 21.
+    Qed.
+
+    Lemma dom_dataD_in_D : dom_rel (data ⨾ ⦗D⦘) ⊆₁ D.
+    Proof.
+      unfold CertExecution2.D.
+      rewrite !id_union; relsf; unionL; splits.
+      { rewrite (data_in_sb WF).
+        generalize dom_sb_covered. basic_solver 21. }
+      { rewrite (data_in_ppo WF).
+        basic_solver 12. }
+      { rewrite (data_in_sb WF).
+        rewrite (dom_l (@wf_sbE G)) at 1.
+        rewrite sb_tid_init' at 1; relsf; unionL; split.
+        { unionR left -> left -> left -> right.
+          unfold same_tid; unfolder; ins; desf; eauto 20. }
+        arewrite (⦗E⦘ ⨾ ⦗fun a : actid => is_init a⦘ ⊆ ⦗D⦘).
+        generalize D_init; basic_solver.
+        arewrite (dom_rel (⦗D⦘ ⨾ sb ⨾ ⦗E ∩₁ NTid_ thread⦘) ⊆₁ D) by basic_solver.
+        unfold CertExecution2.D; basic_solver 12. }
+      { rewrite dom_rel_eqv_dom_rel.
+        rewrite crE at 1; relsf; unionL; splits.
+        { rewrite (dom_r (wf_dataD WF)), (dom_l (@wf_ppoD G)). type_solver. }
+        rewrite (data_in_ppo WF).
+        sin_rewrite ppo_rfi_ppo. basic_solver 21. }
+      { rewrite (dom_r (wf_dataD WF)), (dom_r (wf_rfiD WF)). type_solver. }
+      rewrite (dom_r (wf_dataD WF)), (dom_r (wf_rfeD WF)). type_solver.
+    Qed.
+
+  End CertGraphProperties.
+End CertGraph. 
+
+Section CertGraphLemmas.
+
+Variable prog : Prog.t.
+Variable G  : execution.
+Variable GPROG : program_execution prog G.
+Variable sc : relation actid.
+Variable TC : trav_config.
+Variable TC': trav_config.
+Variable thread : thread_id.
+
+Notation "'E'" := G.(acts_set).
+
+Notation "'R'" := (fun a => is_true (is_r G.(lab) a)).
+Notation "'W'" := (fun a => is_true (is_w G.(lab) a)).
+Notation "'F'" := (fun a => is_true (is_f G.(lab) a)).
+
+Notation "'Rel'" := (fun a => is_true (is_rel G.(lab) a)).
+
+Notation "'R_ex'" := (fun a => R_ex G.(lab) a).
+
+Notation "'sb'" := (G.(sb)).
+Notation "'rmw'" := G.(rmw).
+Notation "'addr'" := G.(addr).
+Notation "'data'" := G.(data).
+Notation "'ctrl'" := G.(ctrl).
+Notation "'rmw_dep'" := G.(rmw_dep).
+Notation "'rf'" := (G.(rf)).
+Notation "'co'" := (G.(co)).
+
+Notation "'ppo'" := (G.(ppo)).
+Notation "'hb'" := (G.(imm_s_hb.hb)).
+Notation "'vf'" := (furr G sc).
+
+Notation "'C'"  := (covered TC).
+Notation "'I'"  := (issued TC).
+Notation "'C''"  := (covered TC').
+Notation "'I''"  := (issued TC').
+
+Notation "'E0'" := (E0 G TC' thread). 
+Notation "'D'" := (D G TC' thread).
+
+Variable WF : Wf G.
+Variable Wf_sc : wf_sc G sc.
+Variable IMMC : imm_consistent G sc.
+Variable TCCOH : tc_coherent G sc TC.
+Variable TSTEP : isim_trav_step G sc thread TC TC'.
+
+Hint Resolve TCCOH'. 
+
+Lemma sim_cert_graph_start 
+      (state : Language.Language.state (Promise.thread_lts thread))
+      (NINITT : thread <> tid_init)
+      (GPC : wf_thread_state thread state)
+      (SSTATE : sim_state G sim_normal C state)
+      (STATECOV : acts_set state.(ProgToExecution.G) ⊆₁ C) :
+  exists state', cert_graph G sc TC TC' thread state'.
+Proof. 
+    cdes SSTATE. cdes SSTATE1.
+
+    assert (wf_thread_state thread state') as GPC'.
+    { eapply wf_thread_state_steps; eauto. }
+
+    assert (forall r w, rmw r w -> covered TC' r <-> covered TC' w) as RMWCOV.
+    { eapply sim_trav_step_rmw_covered; eauto.
+      { red. eauto. }
+      admit. }
+
+    edestruct E0_eindex; eauto; desf. 
+    edestruct steps_middle_set with
+      (thread := thread)
+      (state0 := state) (state':=state') as [state''].
+    3: { eapply E0_eq_certE; eauto. }
+    all: eauto. 
+    { apply set_subset_inter_r. split.
+      { etransitivity. 
+        { eapply steps_preserve_E; eauto. }
+        etransitivity. 
+        { eapply TEH.(tr_acts_set). }
+        basic_solver. }
+      unionR left.
+      etransitivity; eauto.
+      eapply sim_trav_step_covered_le. red. eauto. }
+    { ins.
+      eapply rmw_in_thread_restricted_rmw in RMW; eauto.
+      split; intros [TT XX]; split.
+      1,3: by apply WF.(wf_rmwt) in RMW; rewrite <- TT; red in RMW; desf.
+      all: destruct XX as [XX|XX]; [by left; eapply RMWCOV with (r:=r); eauto|right].
+      all: destruct XX as [e XX].
+      all: apply seq_eqv_r in XX; destruct XX as [SB II].
+      all: exists e; apply seq_eqv_r; split; auto.
+      2: { apply (wf_rmwi WF) in RMW.
+           generalize SB RMW (@sb_trans G). basic_solver. }
+      assert (R r) as RR.
+      { apply WF.(wf_rmwD) in RMW. destruct_seq RMW as [AAA BBB].
+        type_solver. }
+      apply (wf_rmwi WF) in RMW.
+      destruct SB as [|SB]; subst.
+      { eapply issuedW in II; eauto. type_solver. }
+      destruct (classic (w = e)) as [|NEQ]; [by left|].
+      assert (~ is_init r) as NINIT.
+      { intros GG. eapply WF.(init_w) in GG.
+        type_solver. }
+      edestruct sb_semi_total_l with (y:=w) (z:=e); eauto.
+      { apply RMW. }
+      exfalso. eapply RMW; eauto. }
+    desf. 
+
+    assert (wf_thread_state thread state'') as GPC''.
+    { eapply wf_thread_state_steps. apply GPC. auto. }
+    
+    set (new_rf := cert_rf G sc TC' thread ⨾ ⦗ E0 \₁ D ⦘).
+    set (new_rfi := ⦗ Tid_ thread ⦘ ⨾ new_rf ⨾ ⦗ Tid_ thread ⦘).
+    set (new_rfe := ⦗ NTid_ thread ⦘ ⨾ new_rf ⨾ ⦗ Tid_ thread ⦘).
+    set (new_rfe_ex := new_rfe ∪ ⦗ set_compl (codom_rel new_rfe) ⦘).
+
+    assert (new_rfi ⊆ cert_rfi G sc TC' thread) as NEWRFI_IN_CERT. 
+    { unfold cert_rfi. unfold new_rfi, new_rf. basic_solver. }
+
+    assert (new_rff : functional new_rf⁻¹).
+    { arewrite (new_rf ⊆ cert_rf G sc TC' thread).
+      apply cert_rff; auto. }
+    assert (new_rfif : functional new_rfi⁻¹).
+    { arewrite (new_rfi ⊆ new_rf); auto.
+      unfold new_rfi; basic_solver. }
+    assert (new_rfef : functional new_rfe⁻¹).
+    { arewrite (new_rfe ⊆ new_rf); auto.
+      unfold new_rfe; basic_solver. }
+
+    assert (forall r, exists ! w, new_rfe_ex⁻¹ r w) as new_rfe_unique.
+    { ins.
+      destruct (classic ((codom_rel new_rfe) r)) as [X|X].
+      { unfolder in X. 
+        destruct X as [w RFE].
+        exists w; red; splits.
+        unfold new_rfe_ex; basic_solver 12.
+        unfold new_rfe_ex; unfolder; ins; desf.
+        eapply new_rfef; basic_solver.
+        exfalso; eauto. }
+      exists r; red; splits.
+      unfold new_rfe_ex; basic_solver 12.
+      unfold new_rfe_ex; unfolder; ins; desf.
+      unfolder in X; exfalso; eauto. }
+
+    assert (exists new_value, forall x, (new_rfe_ex)⁻¹ x (new_value x)) as HH; desc.
+    { apply (unique_choice (new_rfe_ex)⁻¹ (new_rfe_unique)). }
+
+    set (get_val (v: option value) :=  match v with | Some v => v | _ => 0 end).
+    set (new_val := fun r => get_val (val G.(lab) (new_value r))).
+
+    edestruct steps_old_restrict with (state0:=state'') (state':=state') as [ORMW]; eauto.
+    desc. unnw.
+    edestruct receptiveness_full with
+        (tid:=thread)
+        (s_init:=state) (s:=state'')
+        (new_val:=new_val)
+        (new_rfi:=new_rfi)
+        (MOD:=E0 \₁ D) as [pre_cert_state]; eauto.
+    { red. split; [|basic_solver].  
+      unfold new_rfi, new_rf.
+      rewrite CACTS. 
+      arewrite (
+          ⦗Tid_ thread⦘ ⨾ (cert_rf G sc TC' thread ⨾ ⦗E0 \₁ D⦘) ⨾ ⦗Tid_ thread⦘ ≡ 
+           (cert_rfi G sc TC' thread ⨾ ⦗E0⦘) ⨾ ⦗E0 \₁ D⦘) at 1.
+      { unfold cert_rfi. basic_solver 42. }
+      arewrite (
+          ⦗E0⦘ ⨾ ⦗Tid_ thread⦘ ⨾ cert_rf G sc TC' thread ⨾ ⦗E0 \₁ D⦘ ⨾ ⦗Tid_ thread⦘ ⨾ ⦗E0⦘ ≡
+          ⦗E0⦘ ⨾ cert_rfi G sc TC' thread ⨾ ⦗E0⦘ ⨾ ⦗E0 \₁ D⦘). 
+      { unfold cert_rfi. basic_solver 42. }
+      rewrite <- seqA.
+      rewrite cert_rfi_in_E0; eauto.  
+      basic_solver 10.  
+      admit. }
+      
+    all: admit. 
+    
+    (* { red. split; [|basic_solver].  *)
+    (*   unfold new_rfi, new_rf.  *)
+      
+      
+    (*   apply cert_rfi_in_E0. *)
+    (* { by rewrite CACTS. } *)
+    (* { split; [|basic_solver]. *)
+    (*   rewrite NEW_RFIE at 1. *)
+    (*   unfolder. intros x y [EEX [RFXY EEY]]. *)
+    (*   set (AA := RFXY). *)
+    (*   unfold new_rfi in AA. *)
+    (*   destruct_seq AA as [TX TY]. *)
+    (*   unfold new_rf in AA. apply seq_eqv_r in AA. destruct AA as [AA _]. *)
+    (*   apply cert_rfD in AA. destruct_seq AA as [WX RY]. *)
+    (*   splits; auto; unfold is_w, is_r. *)
+    (*   all: erewrite <- steps_preserve_lab with (state0:=state'') (state':=state'); eauto; *)
+    (*     [by erewrite tr_lab; eauto | | | by apply CACTS]. *)
+    (*   3,4: by rewrite TY; eauto. *)
+    (*   all: by rewrite TX; eauto. } *)
+    (* { rewrite NEWRFISB. unfold Execution.sb. basic_solver. } *)
+    (* { unfold new_rfi, new_rf. basic_solver. } *)
+    (* { rewrite <- CACTS. basic_solver. } *)
+    (* { rewrite STATECOV. *)
+    (*   sin_rewrite sim_trav_step_covered_le. *)
+    (*   2: by red; eauto. *)
+    (*   rewrite <- C_in_D. *)
+    (*   basic_solver. } *)
+    
+
+    
+  
+Admitted.
+
+End CertGraphLemmas.
